data_structure/general_spatial_graph.v
@@ -1,0 +1,75 @@
+Require Import Coq.Sets.Ensembles.
+Require Import Coq.Sets.Finite_sets.
+Require Import VST.msl.seplog.
+Require Import VST.msl.log_normalize.
+Require Import RamifyCoq.Coqlib.
+Require Import RamifyCoq.msl_ext.abs_addr.
+Require Import RamifyCoq.msl_ext.seplog.
+Require Import RamifyCoq.msl_ext.log_normalize.
+Require Import RamifyCoq.msl_ext.iter_sepcon.
+Require Import RamifyCoq.graph.graph_model.
+Require Import RamifyCoq.graph.path_lemmas.
+Require Import RamifyCoq.graph.reachable_computable.
+Require Import RamifyCoq.graph.reachable_ind.
+Require Import RamifyCoq.graph.marked_graph.
+Require Import RamifyCoq.graph.graph_gen.
+Require Import Coq.Logic.Classical.
+Import RamifyCoq.msl_ext.seplog.OconNotation.
+
+Local Open Scope logic.
+
+Class SpatialGraph (V E DV DE: Type): Type := {
+  pg: PreGraph V E;
+  vgamma: V -> DV;
+  egamma: E -> DE
+}.
+
+Arguments vgamma {V E DV DE} _ _.
+Arguments egamma {V E DV DE} _ _.
+
+Class SpatialGraphPred (V E DV DE Pred: Type): Type := {
+  vertex_at: V -> DV -> Pred;
+  edge_at: E -> DE -> Pred
+}.
+
+Class SpatialGraphAssum {V E DV DE Pred: Type} (SGP: SpatialGraphPred V E DV DE Pred) := {
+  SGP_ND: NatDed Pred;
+  SGP_SL : SepLog Pred;
+  SGP_ClSL: ClassicalSep Pred;
+  SGP_CoSL: CorableSepLog Pred
+}.
+
+Existing Instances SGP_ND SGP_SL SGP_ClSL SGP_CoSL.
+
+Class SpatialGraphStrongAssum {V E DV DE Pred: Type} (SGP: SpatialGraphPred V E DV DE Pred) := {
+  SGA: SpatialGraphAssum SGP;
+  SGP_PSL: PreciseSepLog Pred;
+  SGP_OSL: OverlapSepLog Pred;
+  SGP_DSL: DisjointedSepLog Pred;
+  SGP_COSL: CorableOverlapSepLog Pred;
+
+  AAV: AbsAddr V DV;
+  AAE: AbsAddr E DE;
+  VP_MSL: MapstoSepLog AAV vertex_at;
+  VP_sMSL: StaticMapstoSepLog AAV vertex_at;
+  EP_MSL: MapstoSepLog AAE edge_at;
+  EP_sMSL: StaticMapstoSepLog AAE edge_at
+}.
+
+Existing Instances SGA SGP_PSL SGP_OSL SGP_DSL SGP_COSL VP_MSL VP_sMSL EP_MSL EP_sMSL.
+
+Coercion pg : SpatialGraph >-> PreGraph.
+
+Section SpatialGraph.
+
+  Context {V E DV DE Pred: Type}.
+  Context {SGP: SpatialGraphPred V E DV DE Pred}.
+  Context {SGA: SpatialGraphAssum SGP}.
+  Notation Graph := (SpatialGraph V E DV DE).
+
+  Definition graph_cell (g: Graph) (v : V) : Pred := vertex_at v (vgamma g v).
+
+  Definition graph (x : V) (g: Graph) : Pred :=
+    EX l : list V, !!reachable_list g x l && iter_sepcon l (graph_cell g).
+
+End SpatialGraph.
